Proved CDH to SCDH reduction, fixed Hashed ElGamal

examples/CDH.ec
@@ -1,6 +1,6 @@
 require import Int.
 require import Real.
-require import Set_Why.
+require import FSet.
 
 
 (** Minimalist group theory with only needed components *)
@@ -18,9 +18,9 @@ theory Group.
 
   op ( ^ ) : group -> int -> group.
 
-  axiom pow_mult (x, y:int) : (g ^ x) ^ y = g ^ (x * y).
+  axiom pow_mult (x y:int) : (g ^ x) ^ y = g ^ (x * y).
  
-  axiom pow_plus (x, y:int) : (g ^ x) * (g ^ y) = g ^ (x + y).
+  axiom pow_plus (x y:int) : (g ^ x) * (g ^ y) = g ^ (x + y).
 
 end Group.
 
@@ -31,7 +31,7 @@ theory CDH.
   import Group.
 
   module type Adversary = {
-    fun solve(gx:group, gy:group) : group
+    fun solve(gx gy:group) : group {*}
   }.
 
   module CDH (A:Adversary) = {
@@ -53,13 +53,11 @@ end CDH.
 theory Set_CDH.
 
   import Group.
-  import Fset.
-  import FsetNth.
 
   const n : int.
 
   module type Adversary = {
-    fun solve(gx:group, gy:group) : group set
+    fun solve(gx:group, gy:group) : group set {*}
   }.
 
   module SCDH (B:Adversary) = {
@@ -77,13 +75,14 @@ theory Set_CDH.
   module CDH_from_SCDH (A:Adversary) : CDH.Adversary = {
     fun solve(gx:group, gy:group) : group = {
       var s : group set;
-      var i : int;
+      var x : group;
 
       s = A.solve(gx, gy);
-      i = $[0.. card s - 1];
-      return (nth i s);
+      x = $Duni.duni s;
+      return x;
     }
   }.
+
 
   (** Naive reduction to CDH *)
 
@@ -91,53 +90,81 @@ theory Set_CDH.
   lemma nosmt le_compat_r (w x y: real) : 0%r < w => x * w <= y * w => x <= y 
   by [].
 
-  lemma inv_le (x y:real) : 0%r < x => 0%r < y => y <= x => inv x <= inv y.
+  lemma nosmt inv_le (x y:real) : 0%r < x => 0%r < y => y <= x => inv x <= inv y.
   proof.
     intros _ _ _.
     apply (le_compat_r x); first trivial.
     apply (le_compat_r y); first trivial.
     cut H : ((x * inv x) * y <= (y * inv y) * x); last smt.
     rewrite (Inverse y _); first smt.
-    rewrite (Inverse x _); smt.
+    by rewrite (Inverse x _); smt.
   qed.
 
-  lemma nosmt div_le (x y:real) : 
-    0%r < x => 0%r < y => y <= x => 1%r / x <= 1%r / y 
-  by [].
+  lemma div_le (x y:real) : 
+    0%r < x => 0%r < y => y <= x => 1%r / x <= 1%r / y .
+  proof.
+    by progress; cut X := inv_le x y; smt.
+  qed.
 
-  lemma mult_inv_le_r (x y z:real) : 
-    0%r < x => (1%r / x) * y <= z => y <= x * z
-  by [].
+  lemma mu_duni_mem (s:'a set) (x:'a) :
+    mem x s => 1%r / (card s)%r <= mu (Duni.duni s) ((=) x).
+  proof.
+    by intros _; rewrite Duni.mu_def; smt.
+  qed.
 
-  lemma Reduction (A <: Adversary) &m :
+  module SCDH' (A:Adversary) = {
+    var x, y : int
+
+    fun aux() : group set = {
+      var s : group set;
+      x = $[0..q-1];
+      y = $[0..q-1];
+      s = A.solve(g ^ x, g ^ y);
+      return s;
+    }
+
+    fun main() : bool = {
+      var z : group;
+      var s : group set;
+      s = aux();
+      z = $Duni.duni s;
+      return z = g ^ (x * y);
+    }
+  }.
+
+  lemma Reduction (A <: Adversary {SCDH'}) &m :
     0 < n =>
     exists (B <: CDH.Adversary), 
       1%r / n%r * Pr[SCDH(A).main() @ &m : res] <=
       Pr[CDH.CDH(B).main() @ &m : res]. 
   proof.
-    intros n_pos.
-    exists (CDH_from_SCDH(A)).
-    bdhoare_deno (_ : true ==> _); [ | trivial | trivial ].
-    fun; inline CDH_from_SCDH(A).solve; wp.    
-    seq 5 : (mem (g ^ (x * y)) s /\ card s <= n)
-      Pr[SCDH(A).main() @ &m : res] (1%r / n%r) (1%r - (1%r / n%r)) 0%r.
-    by call (_ : true); wp; do rnd; skip; smt.
-    (* This is exactly the SCDH(A) game in the bound *)
-    admit.
-      
-    rnd (lambda i, nth i s = g ^ (x * y)).
-    skip => &m1 H1 //=.
-    apply (Trans _ (1%r / (card s{m1})%r)).
-    apply div_le; smt.
-    apply (mu_choose_mem s{m1} (g ^ (x{m1} * y{m1})) _); first smt. 
-
-    pr_bounded.
-    smt.
+   intros n_pos; exists (CDH_from_SCDH(A)).
+   apply (Trans _ Pr[SCDH'(A).main() @ &m : res]); first last.
+     equiv_deno (_ : true ==> ={res}) => //.
+     fun; inline CDH_from_SCDH(A).solve SCDH'(A).aux.
+     by wp; rnd; wp; call (_:true); wp; do rnd.
+   
+     bdhoare_deno (_ : true ==> _) => //.
+     fun. 
+     seq 1 : (mem (g ^ (SCDH'.x * SCDH'.y)) s /\ card s <= n)
+             Pr[SCDH(A).main() @ &m: res]
+             (1%r / n%r)
+             (1%r - Pr[SCDH(A).main() @ &m: res])
+             0%r => //. 
+       conseq (_ : _ : = (Pr[SCDH(A).main() @ &m : res])).
+       call (_ : true ==> mem (g ^ (SCDH'.x * SCDH'.y)) res /\ card res <= n) => //.
+       bypr; progress.
+       equiv_deno (_: 
+         true ==> 
+         (mem (g ^ (SCDH'.x * SCDH'.y)) res /\ card res <= n){1} = res{2}) => //.
+       fun *; inline SCDH(A).main SCDH'(A).aux; wp.
+       by call (_:true); do rnd; skip; smt.
+       
+       rnd ((=) (g ^ (SCDH'.x * SCDH'.y))).
+       by skip => &m1 H1; split => //; rewrite Duni.mu_def; smt.
   qed.  
 
   (** Shoup's reduction to CDH -- would be nice to prove a bound *)
-
-  import MapFilter.
 
   module CDH_from_SCDH_Shoup (A:Adversary, B:Adversary) : CDH.Adversary = {
     fun solve(gx:group, gy:group) : group = {
@@ -149,7 +176,7 @@ theory Set_CDH.
       a = $[0..q-1];
       b = $[0..q-1];
       s2 = B.solve(gx ^ a * g ^ b, g ^ b);    
-      r = choose (filter (lambda (z:group), mem (z ^ a * gy ^ b) s2) s1);
+      r = pick (filter (lambda (z:group), mem (z ^ a * gy ^ b) s2) s1);
       return r;
     }
   }.
