examples/hashed_elgamal.ec
@@ -1,12 +1,14 @@
 require import Int.
 require import Real.
-require import FMap. import OptionGet.
+require import FMap. 
 require import FSet.
 require import CDH.
 require Logic.
 require AWord.
 require RandOrcl.
 require PKE.
+
+import OptionGet.
 
 
 const k : int.
@@ -30,19 +32,43 @@ type ciphertext = group * bitstring.
 
 op (^^) : bitstring -> bitstring -> bitstring = Bitstring.(^).
 
-op uniform : bitstring distr = Bitstring.Dword.dword.
-
-lemma uniform_total (x:bitstring) : Distr.in_supp x uniform 
-by [].
-
-lemma uniform_spec (x y:bitstring) : Distr.mu_x uniform x = Distr.mu_x uniform y
-by [].
-
 clone import PKE as PKE_ with
   type pkey = pkey,
   type skey = skey,
   type plaintext = plaintext,
   type ciphertext = ciphertext. 
+
+module type Hash = {
+  fun init() : unit
+  fun hash(x:group) : bitstring
+}.
+
+module Hashed_ElGamal (H:Hash) : Scheme = {
+  fun kg() : pkey * skey = {
+    var sk : int;
+    H.init();
+    sk = $[0..q-1];
+    return (g ^ sk, sk);   
+  }
+
+  fun enc(pk:pkey, m:plaintext) : ciphertext = {
+    var y : int;
+    var h : plaintext;
+    y = $[0..q-1];
+    h = H.hash(pk ^ y);
+    return (g ^ y, h ^^ m);
+  }
+
+  fun dec(sk:skey, c:ciphertext) : plaintext option = {
+    var gy : group;
+    var h, hm : bitstring;
+    (gy, hm) = c; 
+    h = H.hash(gy ^ sk);
+    return Option.Some (h ^^ hm); 
+  }
+}.
+
+op uniform : bitstring distr = Bitstring.Dword.dword.
 
 clone import RandOrcl as RandOrcl_group with 
   type from = group,
@@ -52,422 +78,283 @@ clone import RandOrcl as RandOrcl_group with
   op default = Bitstring.zeros.
 
 import ROM.
+import WRO_Set.
 
-(* Using Set_Why *)
-theory WRO_Fset.
-
-  module ARO (R:Oracle) : Oracle = {
-    var log : from set
-
-    fun init() : unit = {
-      R.init();
-      log = FSet.empty;
-    }
-
-    fun o(x:from) : to = {
-      var r : to;
-
-      if (card log < qO) {
-        log = add x log;
-        r = R.o(x);
-      }
-      else r = default;
-      return r;
-    }
-  }.
-
-end WRO_Fset.
-
-import WRO_Fset.
+(* ROM Adversary *)
 
 
-module Hashed_ElGamal (O:Oracle) : Scheme = {
- module AO = ARO(RO)
-  fun kg() : pkey * skey = {
-    var sk : int;
-    AO.init();
-    sk = $[0..q-1];
-    return (g ^ sk, sk);   
-  }
-
-  fun enc(pk:pkey, m:plaintext) : ciphertext = {
-    var y : int;
-    var h : plaintext;
-
-    y = $[0..q-1];
-    h = O.o(pk ^ y);
-    return (g ^ y, h ^^ m);
-  }
-
-  fun dec(sk:skey, c:ciphertext) : plaintext Option.option = {
-    var gy : group;
-    var h, hm : bitstring;
-
-    (gy, hm) = c; 
-    h = O.o(gy ^ sk);
-    return Option.Some (h ^^ hm); 
-  }
-}.
-
-
-module type Adv (O:ARO) = {
-  fun choose(pk:pkey)     : plaintext * plaintext
+module type Adversary (O:ARO) = {
+  fun choose(pk:pkey)     : plaintext * plaintext {* O.o}
   fun guess(c:ciphertext) : bool
 }.
 
+module AO = ARO(RO).
 
-module G1 (A_:Adv) = { 
-  module S = Hashed_ElGamal(RO)
-  module AO = ARO(RO)
-  module A = A_(AO)
-  
-  var gxy : group
-
-  fun main() : bool = {
-    var x, y : int;
-    var gx : group;
-    var m0, m1 : plaintext;
-    var c : ciphertext;
-    var b, b' : bool;
-    var h, z : bitstring;
-
-    AO.init();
-    x       = $[0..q-1];
-    y       = $[0..q-1];
-    gx      = g ^ x; 
-    gxy     = gx ^ y;
-    (m0,m1) = A.choose(gx);
-    b       = ${0,1};
-    h       = $uniform;
-    c       = (g ^ y, h ^^ (b ? m1 : m0));
-    b'      = A.guess(c);
-    return (b' = b);
-  }
+module H : Hash = {
+  fun init() : unit = { AO.init(); }
+  fun hash(x:group) : bitstring = { var y : bitstring; y = RO.o(x); return y; }
 }.
 
+module S = Hashed_ElGamal(H).
 
-lemma CPA_G1 (A <: Adv {CPA, G1, RO, ARO, Hashed_ElGamal}) :
-  (forall (O <: ARO), islossless O.o => islossless A(O).choose) =>
-  (forall (O <: ARO), islossless O.o => islossless A(O).guess) =>
-  equiv 
-  [ CPA(Hashed_ElGamal(RO), A(ARO(RO))).main ~ G1(A).main : 
-    (glob A){1} = (glob A){2} ==> !(mem G1.gxy ARO.log){2} => ={res} ].
-proof.
-  intros Hll1 Hll2; fun.
-  inline ARO(RO).init G1(A).AO.init RO.init 
-    Hashed_ElGamal(RO).kg Hashed_ElGamal(RO).enc Hashed_ElGamal(RO).AO.init.
-  swap{1} 9 -5.
-  seq 5 6 : 
-    ((glob A){1} = (glob A){2} /\ ={ARO.log, RO.m, y} /\
-     RO.m{1} = FMap.Core.empty /\ ARO.log{2} = FSet.empty /\
-     pk{1} = gx{2} /\ (G1.gxy = gx ^ y){2}).
-  wp; do rnd; wp; skip; progress; try smt.
-  seq 2 2 : 
-    ((glob A){1} = (glob A){2} /\ ={ARO.log, RO.m, y, b, m0, m1} /\
-     pk{1} = gx{2} /\ (G1.gxy = gx ^ y){2} /\
-     (forall x, mem x ARO.log <=> in_dom x RO.m){2}).
+section.
 
-  rnd.
-  call (_ : ={RO.m, ARO.log} /\ (forall x, mem x ARO.log <=> in_dom x RO.m){2}).
-  fun; inline RO.o; wp; if; first smt.
-  by wp; rnd; wp; skip; progress; smt (* may timeout *).
-  by wp; skip; smt.
-  by skip; smt.
+  declare module A_ : Adversary {RO, ARO, SCDH.SCDH'}.
 
-  call (_ : (mem G1.gxy ARO.log), 
-       (={ARO.log} /\ eq_except RO.m{1} RO.m{2} G1.gxy{2})) => //.
-  by intros O _; apply (Hll2 O) => //.
-  fun; inline RO.o; wp; if; first smt.
-  wp; rnd; wp; skip; progress=> //; first 5 last; last 6 smt.
-  case (x = G1.gxy){2}; first smt.
-  cut em: forall a, a => !a => false by smt=> //.
-  by cut:= em (in_dom x{2} RO.m{2}) _ _=> //; smt.
-  by wp; skip; smt.
+  axiom lossless_choose (O <: ARO) : islossless O.o => islossless A_(O).choose.
 
-  intros _ _; fun; if; inline RO.o; wp.
-  by rnd Fun.cpTrue; wp; skip; smt.
-  by wp; skip; smt.
+  axiom lossless_guess (O <: ARO) : islossless O.o => islossless A_(O).guess.
+
+  local module A = A_(AO).
+
+  local module G1 = { 
+    var gxy : group
+
+    fun main() : bool = {
+      var x, y : int;
+      var gx : group;
+      var m0, m1 : plaintext;
+      var c : ciphertext;
+      var b, b' : bool;
+      var h, z : bitstring;   
+      AO.init();
+      x       = $[0..q-1];
+      y       = $[0..q-1];
+      gx      = g ^ x; 
+      gxy     = gx ^ y;
+      (m0,m1) = A.choose(gx);
+      b       = ${0,1};
+      h       = $uniform;
+      c       = (g ^ y, h ^^ (b ? m1 : m0));
+      b'      = A.guess(c);
+      return (b' = b);
+    }
+  }.
+
+  local equiv CPA_G1 :
+    CPA(S, A).main ~ G1.main : true ==> !(mem G1.gxy ARO.log){2} => ={res}.
+  proof.
+    fun.
+    inline AO.init RO.init H.init Hashed_ElGamal(H).kg Hashed_ElGamal(H).enc.
+    swap{1} 9 -5.
+    seq 5 6 : 
+      (={ARO.log, RO.m, y} /\
+       RO.m{1} = FMap.Core.empty /\ ARO.log{2} = FSet.empty /\
+       pk{1} = gx{2} /\ (G1.gxy = gx ^ y){2}); first by wp; do rnd; wp.
+    seq 2 2 : 
+      (={glob A, ARO.log, RO.m, y, b, m0, m1} /\
+       pk{1} = gx{2} /\ (G1.gxy = gx ^ y){2} /\
+       (forall x, mem x ARO.log <=> in_dom x RO.m){2}).   
+      rnd.
+      call (_ : ={RO.m, ARO.log} /\ (forall x, mem x ARO.log <=> in_dom x RO.m){2}).
+        fun; inline RO.o; wp; if; first by smt.
+          by wp; rnd; wp; skip; progress; smt.
+          by wp.
+      by skip; smt.
+
+      call (_ : (mem G1.gxy ARO.log), 
+                (={ARO.log} /\ eq_except RO.m{1} RO.m{2} G1.gxy{2})) => //.
+        by intros O; apply (lossless_guess O).
+   
+        fun; inline RO.o; wp; if; first smt.
+        wp; rnd; wp; skip; progress=> //; first 5 last; last 6 smt.
+        by case (x = G1.gxy){2}; smt.
+        by wp.
+       
+        intros _ _; fun; if; inline RO.o; wp.
+        by rnd; wp; skip; smt.
+        by wp.
+        
+        intros _; fun; if; inline RO.o; wp.
+        by rnd; wp; skip; smt.
+        by wp.
+
+      by inline H.hash RO.o; wp; rnd; wp; skip; progress; smt.
+  qed.
+
+  local module G2 = {
+    var gxy : group
+   
+    fun main() : bool = {
+      var x, y : int;
+      var gx : group;
+      var m0, m1 : plaintext;
+      var c : ciphertext;
+      var b, b' : bool;
+      var h, z : bitstring;
+      AO.init();
+      x        = $[0..q-1];
+      y        = $[0..q-1];
+      gx       = g ^ x; 
+      gxy      = gx ^ y;
+      (m0,m1)  = A.choose(gx);
+      h        = $uniform;
+      c        = (g ^ y, h);
+      b'       = A.guess(c);
+      b        = ${0,1};
+      return (b' = b);
+    }
+  }.
+   
+   
+  local equiv G1_G2 :
+     G1.main ~ G2.main : true ==> ={res, ARO.log} /\ G1.gxy{1} = G2.gxy{2}.
+  proof.
+    fun.
+    inline AO.init RO.init.
+    swap{2} 11 -3.
+    call (_ : ={ARO.log, RO.m} /\ G1.gxy{1} = G2.gxy{2}).
+      fun; inline RO.o; wp; if; first smt.
+        by wp; rnd; wp; skip; smt.
+        by wp.
+    wp.
+    rnd (lambda h, h ^^ if b then m1 else m0){1}; rnd.
+    call ( _ : ={ARO.log, RO.m} /\ G1.gxy{1} = G2.gxy{2}).
+    fun; inline RO.o; wp; if; first smt.
+      by wp; rnd; wp; skip; smt.
+      by wp.
+    wp; do rnd; wp; skip; progress=> //; smt.
+  qed.
+   
+  local module SCDH_from_CPA : SCDH.Adversary = {
+    fun solve(gx:group, gy:group) : group set = {
+      var m0, m1 : plaintext;
+      var h : bitstring;
+      var b' : bool;
+      AO.init();
+      (m0,m1)  = A.choose(gx);
+      h        = $uniform;
+      b'       = A.guess((gy, h));
+      return ARO.log;
+    }
+  }.
+   
+  local equiv G2_SCDH :
+    G2.main ~ SCDH.SCDH(SCDH_from_CPA).main : 
+    true ==> (mem G2.gxy ARO.log){1} = res{2} /\ card ARO.log{1} <= qH.
+  proof.
+    fun.
+    inline SCDH_from_CPA.solve AO.init RO.init.
+    swap{2} [5..6] -4.  
+    rnd{1}; wp.  
+    seq 9 8 : 
+      ((glob A){1} = (glob A){2} /\ ={ARO.log, RO.m} /\
+      c{1} = (gy, h){2} /\ G2.gxy{1} = g ^ (x * y){2} /\ card ARO.log{1} <= qH).
+      wp; rnd; call ( _ : ={ARO.log, RO.m} /\ card ARO.log{1} <= qH).
+      fun; inline RO.o; wp; if; first by smt.
+        by wp; rnd; wp; skip; smt.
+        by wp.
+      by wp; do rnd; wp; skip; smt.
+   
+      call ( _ :
+       RO.m{1} = RO.m{2} /\ ARO.log{1} = ARO.log{2} /\ card ARO.log{1} <= qH).
+        fun; inline RO.o; wp; if; first smt.
+          by wp; rnd; wp; skip; smt.
+          by wp.
+        by skip; smt.
+  qed.
+      
+  local lemma Pr_CPA_G1 &m :
+    Pr[CPA(S, A).main() @ &m : res] <=
+    Pr[G1.main() @ &m : res \/ mem G1.gxy ARO.log]. 
+  proof.
+    by equiv_deno CPA_G1 => //; smt.
+  qed.
+      
+  local lemma Pr_G1_G1 &m :
+    Pr[G1.main() @ &m : res \/ mem G1.gxy ARO.log] <=
+    Pr[G1.main() @ &m : res] + Pr[G1.main() @ &m : mem G1.gxy ARO.log].
+  proof.
+    apply (Trans _
+      (Pr[G1.main() @ &m : res] + 
+       Pr[G1.main() @ &m : mem G1.gxy ARO.log] -
+       Pr[G1.main() @ &m : res /\ mem G1.gxy ARO.log])).
+    cut W: (forall (x y:real), x = y => x <= y) by smt.
+    by apply W; rewrite Pr mu_or; smt.
+    by smt.
+  qed.
+   
+  local lemma Pr_G1_G2_res &m : 
+    Pr[G1.main() @ &m : res] = Pr[G2.main() @ &m : res].
+  proof.
+    by equiv_deno G1_G2=> //; smt.
+  qed.
+      
+  local lemma Pr_G1_G2_mem &m : 
+    Pr[G1.main() @ &m : mem G1.gxy ARO.log] = 
+    Pr[G2.main() @ &m : mem G2.gxy ARO.log].
+  proof.
+    by equiv_deno G1_G2=> //; smt.
+  qed.
   
-  intros _; fun; if; inline RO.o; wp.
-  by rnd Fun.cpTrue; wp; skip; smt.
-  by wp; skip; smt.
-  
-  by inline RO.o; wp; rnd; wp; skip; progress; smt.
-qed.
+  local lemma Pr_G2 &m : Pr[G2.main() @ &m : res] = 1%r / 2%r.
+  proof.
+    bdhoare_deno (_ : true ==> _) => //.
+    fun; rnd ((=) b').
+    call (_ : true) => //.
+    by intros => O _; apply (lossless_guess O).
+    by apply RO_lossless_o; smt.
+    wp; rnd; call (_ : true).
+    by intros => O _; apply (lossless_choose O).
+    by apply RO_lossless_o; smt.
+    by wp; do rnd; inline AO.init RO.init; wp; skip; progress; smt.
+  qed.
+      
+  local lemma Pr_G2_SCDH &m : 
+    Pr[G2.main() @ &m : mem G2.gxy ARO.log] =
+    Pr[SCDH.SCDH(SCDH_from_CPA).main() @ &m : res].
+  proof.
+    by equiv_deno G2_SCDH.
+  qed.
+   
+  local lemma Reduction &m :
+    Pr[CPA(S, A).main() @ &m : res] <=
+    1%r / 2%r + Pr[SCDH.SCDH(SCDH_from_CPA).main() @ &m : res].
+  proof. 
+    apply (Trans _ Pr[G1.main() @ &m : res \/ mem G1.gxy ARO.log]);
+    first by apply (Pr_CPA_G1 &m).
+    apply (Trans _
+      (Pr[G1.main() @ &m : res] + Pr[G1.main() @ &m : mem G1.gxy ARO.log])).
+    by apply (Pr_G1_G1 &m).
+    by rewrite (Pr_G1_G2_res &m) (Pr_G2 &m) (Pr_G1_G2_mem &m) (Pr_G2_SCDH &m).
+  qed.
+   
+  local lemma Security_SCDH &m :
+    exists (B <: SCDH.Adversary {SCDH.SCDH'}),
+      Pr[CPA(S, A).main() @ &m : res] - 1%r / 2%r <= 
+      Pr[SCDH.SCDH(B).main() @ &m : res].
+  proof.
+    exists SCDH_from_CPA.
+    cut W : forall (x y z : real), x <= z + y => x - z <= y by smt.
+    by apply W; apply (Reduction &m).
+  qed.
+   
+  lemma mult_inv_le_r (x y z:real) : 
+    0%r < x => (1%r / x) * y <= z => y <= x * z
+  by [].
 
+  (** Composing reduction from CPA to SCDH with reduction from SCDH to CDH *)
+  lemma Security &m :
+    exists (B <: CDH.Adversary),
+      Pr[CPA(S, A_(AO)).main() @ &m : res] - 1%r / 2%r <= 
+      qH%r * Pr[CDH.CDH(B).main() @ &m : res].
+  proof.
+    elim (Security_SCDH &m) => B H.
+    elim (SCDH.Reduction B &m _); first by smt.
+    intros C H1; exists C.
+    apply (Trans _ Pr[SCDH.SCDH(B).main() @ &m : res]) => //.
+    by apply mult_inv_le_r; first smt.
+  qed.
+     
+  lemma Correctness : 
+    hoare [Correctness(S).main : true ==> res].
+  proof.
+    fun.
+    inline Hashed_ElGamal(H).kg Hashed_ElGamal(H).enc Hashed_ElGamal(H).dec.
+    inline H.hash RO.o H.init AO.init RO.init.
+    by do (wp; rnd); wp; skip; progress; smt.
+  qed.
 
-module G2 (A_:Adv) = { 
-  module S  = Hashed_ElGamal(RO)
-  module AO = ARO(RO)
-  module A  = A_(AO)
-  
-  var gxy : group
+end section.
 
-  fun main() : bool = {
-    var x, y : int;
-    var gx : group;
-    var m0, m1 : plaintext;
-    var c : ciphertext;
-    var b, b' : bool;
-    var h, z : bitstring;
-
-    AO.init();
-    x        = $[0..q-1];
-    y        = $[0..q-1];
-    gx       = g ^ x; 
-    gxy      = gx ^ y;
-    (m0,m1)  = A.choose(gx);
-    h        = $uniform;
-    c        = (g ^ y, h);
-    b'       = A.guess(c);
-    b        = ${0,1};
-    return (b' = b);
-  }
-}.
-
-
-lemma G1_G2 (A <: Adv {G1, G2, RO, ARO, Hashed_ElGamal}) :
-  equiv 
-  [ G1(A).main ~ G2(A).main : 
-    (glob A){1} = (glob A){2} ==> ={res, ARO.log} /\ G1.gxy{1} = G2.gxy{2} ].
-proof.
-  fun.
-  inline G1(A).AO.init G2(A).AO.init RO.init.
-  swap{2} 11 -3.
-  call (_ : ={ARO.log, RO.m} /\ G1.gxy{1} = G2.gxy{2}).
-
-  fun; inline RO.o; wp; if; first smt.
-  by wp; rnd; wp; skip; smt.
-  by wp; skip; smt.
-  wp.
-  rnd (lambda h, h ^^ if b then m1 else m0){1}
-      (lambda h, h ^^ if b then m1 else m0){1}.
-  rnd.
-  call ( _ : ={ARO.log, RO.m} /\ G1.gxy{1} = G2.gxy{2}).
-  fun; inline RO.o; wp; if; first smt.
-  by wp; rnd; wp; skip; smt.
-  by wp; skip; smt.
-  wp; do rnd; wp; skip; progress=> //;first 2 by smt.
-  by generalize (if bL then x2 else x1) => x; smt.
-  by generalize (if bL then x2 else x1) => x; smt.
-qed.
-
-(** The following is no longer in synch because of the use of Set_why... We can no longer maintain this example. *)
-module SCDH_from_CPA (A_:Adv) : SCDH.Adversary = {
-  module AO = ARO(RO)
-  module A  = A_(AO)
-
-  fun solve(gx:group, gy:group) : group set = {
-    var m0, m1 : plaintext;
-    var h : bitstring;
-    var b' : bool;
-
-    AO.init();
-    (m0,m1)  = A.choose(gx);
-    h        = $uniform;
-    b'       = A.guess((gy, h));
-    return ARO.log;
-  }
-}.
-
-(*
-Already in Why3
-
-lemma subset_card (s1 s2:'a set) : s1 <= s2 => #s1 <= #s2
-by [].
-
-lemma add_subset (x:'a) (s:'a set) : s <= add x s
-by [].
-
-lemma add_card_notmem (x:'a) (s:'a set) : !mem x s => #add x s = #s + 1
-by [].
-
-lemma add_card_mem (x:'a) (s:'a set) : mem x s => #s = 1 + #remove x s
-by [].
-*)
-
-lemma add_mem (x:'a) (s:'a set) : mem x s => add x s = s
-by (intros _; apply extensionality; smt).
-
-lemma card_add (x:'a) (s:'a set) : card (add x s) <= card s + 1
-by [].
-
-
-lemma G2_SCDH (A <: Adv {CPA, G1, G2, SCDH.SCDH, RO, ARO, Hashed_ElGamal}) :
-  (forall (O <: ARO), islossless O.o => islossless A(O).choose) =>
-  (forall (O <: ARO), islossless O.o => islossless A(O).guess) =>
-  equiv 
-  [ G2(A).main ~ SCDH.SCDH(SCDH_from_CPA(A)).main : 
-    (glob A){1} = (glob A){2} ==> 
-    (mem G2.gxy ARO.log){1} = res{2} /\ card ARO.log{1} <= qH ].
-proof.
-  intros _ _; fun.
-  inline SCDH_from_CPA(A).solve SCDH_from_CPA(A).AO.init G2(A).AO.init RO.init.
-  swap{2} [5..6] -4.  
-  rnd{1}; wp.  
-  seq 9 8 : 
-    ((glob A){1} = (glob A){2} /\ ={ARO.log, RO.m} /\
-    c{1} = (gy, h){2} /\ G2.gxy{1} = g ^ (x * y){2} /\ card ARO.log{1} <= qH).
-  wp; rnd.
-  call ( _ : ={ARO.log, RO.m} /\ card ARO.log{1} <= qH).
-  fun; inline RO.o; wp; if; first smt.
-  by wp; rnd; wp; skip; smt.
-  by wp; skip; smt.
-  by wp; do rnd; wp; skip; smt.
-
-  call ( _ : RO.m{1} = RO.m{2} /\ ARO.log{1} = ARO.log{2} /\ card ARO.log{1} <= qH).
-
-  fun; inline RO.o; wp; if; first smt.
-  by wp; rnd; wp; skip; smt.
-  by wp; skip; smt.
-  by skip; smt.
-qed.
-
-
-lemma Pr_CPA_G1 (A <: Adv {CPA, G1, G2, SCDH.SCDH, RO, ARO, Hashed_ElGamal}) &m :
-  (forall (O <: ARO), islossless O.o => islossless A(O).choose) =>
-  (forall (O <: ARO), islossless O.o => islossless A(O).guess) =>
-  Pr[CPA(Hashed_ElGamal(RO), A(ARO(RO))).main() @ &m : res] <=
-  Pr[G1(A).main() @ &m : res \/ mem G1.gxy ARO.log]. 
-proof.
-  intros _ _.
-  equiv_deno (CPA_G1 (A) _ _);try assumption; try smt.
-qed.
-
-
-lemma Pr_G1_G1 (A <: Adv {CPA, G1, G2, SCDH.SCDH, RO, ARO, Hashed_ElGamal}) &m : 
-  (forall (O <: ARO), islossless O.o => islossless A(O).choose) =>
-  (forall (O <: ARO), islossless O.o => islossless A(O).guess) =>
-  Pr[G1(A).main() @ &m : res \/ mem G1.gxy ARO.log] <=
-  Pr[G1(A).main() @ &m : res] + Pr[G1(A).main() @ &m : mem G1.gxy ARO.log].
-proof.
-  intros _ _. 
-  apply (Trans 
-    Pr[G1(A).main() @ &m : res \/ mem G1.gxy ARO.log]
-    (Pr[G1(A).main() @ &m : res] + 
-     Pr[G1(A).main() @ &m : mem G1.gxy ARO.log] -
-     Pr[G1(A).main() @ &m : res /\ mem G1.gxy ARO.log])
-    (Pr[G1(A).main() @ &m : res] + Pr[G1(A).main() @ &m : mem G1.gxy ARO.log]) 
-     _ _).
-  cut W: (forall (x y:real), x = y => x <= y); first smt.
-  by apply W; rewrite Pr mu_or; smt.
-  smt.
-qed.
-
-lemma Pr_G1_G2_res (A <: Adv {CPA, G1, G2, SCDH.SCDH, RO, ARO, Hashed_ElGamal}) &m : 
-  Pr[G1(A).main() @ &m : res] = Pr[G2(A).main() @ &m : res].
-proof.
-  equiv_deno (G1_G2 (A)); smt.
-qed.
-
-
-lemma Pr_G1_G2_mem (A <: Adv {CPA, G1, G2, SCDH.SCDH, RO, ARO, Hashed_ElGamal}) &m : 
-  Pr[G1(A).main() @ &m : mem G1.gxy ARO.log] = 
-  Pr[G2(A).main() @ &m : mem G2.gxy ARO.log].
-proof.
-  equiv_deno (G1_G2 (A)); smt.
-qed.
-
-
-lemma islossless_AO : islossless ARO(RO).o.
-proof.
-  fun; inline ARO(RO).o RO.o; wp; if; wp.
-  by rnd Fun.cpTrue; wp; skip; smt.
-  by skip; trivial.
-qed.
-
-
-lemma Pr_G2 (A <: Adv {CPA, G1, G2, SCDH.SCDH, RO, ARO, Hashed_ElGamal}) &m : 
-  (forall (O <: ARO), islossless O.o => islossless A(O).choose) =>
-  (forall (O <: ARO), islossless O.o => islossless A(O).guess) =>
-  Pr[G2(A).main() @ &m : res] = 1%r / 2%r.
-proof.
-  intros Hll1 Hll2.
-  bdhoare_deno (_ : true ==> _); [ | trivial | trivial ].
-  fun; rnd ((=) b').
-  call (_ : true) => //.
-  by intros => O _;apply (Hll2 O) => //.
-  by apply islossless_AO.
-  wp; rnd Fun.cpTrue; call (_ : true).
-  by intros => O _;apply (Hll1 O) => //.
-  by apply islossless_AO.
-  by wp; do rnd Fun.cpTrue; inline G2(A).AO.init RO.init; wp; skip; progress; smt.
-qed.
-
-
-lemma Pr_G2_SCDH (A <: Adv {CPA, G1, G2, SCDH.SCDH, RO, ARO, Hashed_ElGamal}) &m : 
-  (forall (O <: ARO), islossless O.o => islossless A(O).choose) =>
-  (forall (O <: ARO), islossless O.o => islossless A(O).guess) =>
-  Pr[G2(A).main() @ &m : mem G2.gxy ARO.log] =
-  Pr[SCDH.SCDH(SCDH_from_CPA(A)).main() @ &m : res].
-proof.
-  intros _ _.
-  equiv_deno (G2_SCDH (A) _ _); try assumption;trivial.
-qed.
-
-
-lemma Reduction (A <: Adv {CPA, G1, G2, SCDH.SCDH, RO, ARO, Hashed_ElGamal}) &m :  
-  (forall (O <: ARO), islossless O.o => islossless A(O).choose) =>
-  (forall (O <: ARO), islossless O.o => islossless A(O).guess) =>
-  Pr[CPA(Hashed_ElGamal(RO), A(ARO(RO))).main() @ &m : res] <=
-  1%r / 2%r + Pr[SCDH.SCDH(SCDH_from_CPA(A)).main() @ &m : res].
-proof. 
-  intros _ _.  
-  apply (Trans _ Pr[G1(A).main() @ &m : res \/ mem G1.gxy ARO.log]).
-  by apply (Pr_CPA_G1 (A) &m); assumption.
-  apply (Trans _
-    (Pr[G1(A).main() @ &m : res] + Pr[G1(A).main() @ &m : mem G1.gxy ARO.log])).
-  by apply (Pr_G1_G1 (A) &m); try assumption.
-  rewrite (Pr_G1_G2_res (A) &m).
-  rewrite (Pr_G2 (A) &m); try assumption. 
-  rewrite (Pr_G1_G2_mem (A) &m).  
-  rewrite (Pr_G2_SCDH (A) &m); try assumption.
-  by apply Refl.
-qed.
-
-lemma Security (A <: Adv {CPA, G1, G2, SCDH.SCDH, RO, ARO, Hashed_ElGamal}) &m :
-  (forall (O <: ARO), islossless O.o => islossless A(O).choose) =>
-  (forall (O <: ARO), islossless O.o => islossless A(O).guess) =>
-  exists (B <: SCDH.Adversary),
-    Pr[CPA(Hashed_ElGamal(RO), A(ARO(RO))).main() @ &m : res] - 1%r / 2%r <= 
-    Pr[SCDH.SCDH(B).main() @ &m : res].
-proof.
-  intros _ _.
-  exists ( SCDH_from_CPA(A)).
-  cut W : (forall (x y z : real), x <= z + y => x - z <= y); first smt.
-  by apply W; apply (Reduction (A) &m); assumption.
-qed.
-
-
-(** Composing reduction from CPA to SCDH with reduction from SCDH to CDH *)
-lemma Security_CDH 
-  (A <: Adv {CPA, G1, G2, SCDH.SCDH, RO, ARO, Hashed_ElGamal}) &m :
-  (forall (O <: ARO), islossless O.o => islossless A(O).choose) =>
-  (forall (O <: ARO), islossless O.o => islossless A(O).guess) =>
-  exists (B <: CDH.Adversary),
-    Pr[CPA(Hashed_ElGamal(RO), A(ARO(RO))).main() @ &m : res] - 1%r / 2%r 
-    <= qH%r * Pr[CDH.CDH(B).main() @ &m : res].
-proof.
-  intros _ _.
-  elim (Security (A) &m _ _); try assumption.
-  intros B _.
-  elim (SCDH.Reduction (B) &m _); first smt.
-  intros C _.
-  exists (C).
-  apply (Trans _ Pr[SCDH.SCDH(B).main() @ &m : res]).
-  assumption.
-  apply SCDH.mult_inv_le_r; first smt.
-  assumption.
-qed.
-
-
-lemma Correctness : 
-  hoare [Correctness(Hashed_ElGamal(RO)).main : true ==> res].
-proof.
-  fun.
-  inline Hashed_ElGamal(RO).kg Hashed_ElGamal(RO).enc Hashed_ElGamal(RO).dec. 
-  inline RO.o RO.init Hashed_ElGamal(RO).AO.init.
-  do (wp; rnd); wp; skip; progress; [smt | | smt | smt].
-    cut ->: g ^ y2 ^ sk0 = g ^ sk0 ^ y2; first smt.
-    rewrite Map.get_setE Option.proj_some; smt.
-qed.
+print axiom Security.
